%\href{url}{txt}
\subsection{QR given factorization}
For any $X\in\mathbb{N}$ denote: $QR(X)$ as the set of quadratic residues modulus $X$.\\
Lemma I;
\[
	\forall P,Q\in\mathbb{P}:QR(N)=QR(P)\cap QR(Q)
\]
Proof Lemma I:\\
Let $a\in QR(N)$.
\[
	\exists x,K: x^2\eq_N a
	\Rightarrow x^2=a+(K)PQ
\]\[
	\Rightarrow x^2=a+(KP)Q\wedge x^2=a+(KQ)P
\]\[
	\Rightarrow x^2\eq_Qa\wedge x^2\eq_Pa
\]\[
	\Rightarrow a\in QR(Q)\wedge a\in QR(P)
	\Rightarrow a\in QR(Q)\cap QR(P)
\]
Let $a\in QR(P)\cap QR(Q)$.
Thus:
\[
	\exists x_1,x_2: a\eq_Px_1\wedge a\eq_Qx_2	
\]
Thanks to the
\href{https://en.wikipedia.org/wiki/Chinese_remainder_theorem}
{Chinese remainder theorem}
we know there exists a solution $x$ which satisfies:
\[
	x\eq_Px_1,x\eq_Qx_2
\]
Thus:
\[
	\Rightarrow a\eq_Px^2,a\eq_Qx^2
	\Rightarrow a\eq_{PQ}x^2
	\Rightarrow a\in QR(N)
\]

Now we use the correctness of the Lemma I to define a polynomial algorithm:
\lstinputlisting[language=Python]{code/qr_given_factor.py}

Indeed the names of the variables at lines 4 and 5 are informative (and correct) due
to the properties of Euiler's criterion as seen in class, meaining that
$a$ is qr modulus $P$ iff $a^{(P-1)/2}\eq_P1$, and same with $Q$.\\
This together with Lemma I proves the correctness of this algorithm.\\

We have seen in the last homework how modulus exponantiation can be done efficiently;
which makes this algorithm polynomial.

\subsection{Generating QR}
In the following, all expressions and operations are in the $\mathbb{Z}_N^*$ group
unless said otherwise.\\

Let $x\in QNR(N)$.\\
Lemma I; $x,z\in QNR(N)\Rightarrow zx^{-1}\in QR(N)$:\\
Since $QNR(N)=QNR(P)\cap QNR(Q)$ we get:
\[
	(zx^{-1})^{\frac{p-1}{2}}
	\eq_P(z)^{\frac{p-1}{2}}(x^{-1})^{\frac{p-1}{2}}
	\eq_P(z)^{\frac{p-1}{2}}(x^{\frac{p-1}{2}})^{-1}
	\eq_P(-1)(-1)^{-1}=1
\]
and in the same way under modulus $Q$ we get $(zx^{-1})^{\frac{p-1}{2}}\eq_Q1$.
From Euile's criterion we get that $(zx^{-1})^{\frac{p-1}{2}}\in QR(N)$.\\

Lemma II; $\{y^2x:y\in\mathbb{Z}_N^*\}\supseteq QNR(N)$:\\
Let $z\in QNR(N)$, from Lemma I we get $x^{-1}z\in QR(N)$
Thus:
\[
	\exists y: y^2=zx^{-1}
	\Rightarrow y^2x=z
	\Rightarrow z\in\{y^2x:y\in\mathbb{Z}_N^*\}	
\]

Lemma III; $\{y^2x:y\in\mathbb{Z}_N^*\}\subseteq QNR(N)$:\\
Let $y\in\mathbb{Z}_N^*$. Assume $\exists z:z^2=y^2x$.
Thus:
\[
	z^2y^{-2}=x\Rightarrow (zy^{-1})^2=x\Rightarrow x\notin QNR(N)
\]
Hence the assumption is incorrect, and $y^2x\in QNR(N)$.\\

Proof:\\
Define $g(z)=z\cdot x$, $g:QR(N)\longrightarrow QNR(N)$.\\
From Lemma II and III, we get that $g$'s image is exactly $QNR(N)$.\\
$g$ is invertible and thus is a bijection.\\
Let:
\[
	a^2\in QR(N),\;y\aprx^\$\mathbb{Z}_N^*
\]
Since $y^2$ has four different roots:
\[
	\pr_{y\leftarrow \mathbb{Z}_N^*}[y^2=a^2]
	=\frac{4}{|\mathbb{Z}_N^*|}
	=\frac{1}{\frac{|\mathbb{Z}_N^*|}{4}}
	=\frac{1}{|QR(N)|}
\]
\[
	\Rightarrow y^2\aprx^\$QR(N)
\]
And since $g$ is bijection $QR(N)\rightarrow QNR(N)$:
\[
	g(y^2)=y^2x\aprx^\$ QNR(N)
\]
\[\square\]

\subsection{Public-key Encryption}
The main idea:\\
If factoring primes and QR are hard (without factorization), generate two primes, use
their product as the public key, and their tuple as private key.
Now this 'private key' can be used as a 'cheat' for solving
QR problems; anyone that wants to break the cypher will either
have to find QR without factorization or manage to factor
the primes from the public key:
\lstinputlisting[language=Python]{code/qr_pke.py}

For complexity purposes, assume $n$ is given in unary format.

\subsection{Malleability}
Given two cyphers $c_1,c_2$ encrypted under $N$,
we can return $c_1\cdot c_2$.\\
We need to show that if $b_1,b_2$ are the 
original bits, then:
\[
	Decrypt(c_1\cdot c_2)=XOR(b_1,b_2)
\]
Since we defined our cypher to be QR in the case that
the plaintext is 0, and QNR otherwise,
than this is equivalent to proving that
$c_1\cdot c_2$ is QNR iff exactly one of the
bits $b_1,b_2$ is on.\\
Taking this further; the question is equivalent to 
showing that $c_1\cdot c_2$ is QNR iff exactly one out 
of the pair $c_1, c_2$ is QR.\\

Let $c_1\cdot c_2\in QR$.\\
if both are QR, then:
\[
	c_1=y_1^2,c_2=y_2^2	
\]
\[
	c_1c_2=y_1^2y_2^2=(y_1y_2)^2\in QR	
\]
if both are QNR then:\\
Assume that $x_1\cdot x_2\in QNR$. Than from Lemma II 
in section 1.2: $y^2x=x_1x_2$, thus $x^{-1}x_1x_2$ is 
QR, contredicting Lemma I.
So $x_1x_2\in QR$.\\

if $x_1\in QR, x_2\in QNR$ (oppesite case symmetrical);
than $x_1x_2=y^2x_2\in QR$ from Lemma III.

\subsection{}
Our algorithm will simply take the input cypher $c$, public key $N$,
uniformly sample $z$ from ${1...N}$, and return $z^2\cdot c$.
This works because, as we have seen in section 1.2 multiplying QNR by QR
results with QNR, and as we have seen in section 1.4; multiplying QR by QR 
results with a QR. This means that after our operation the cypher
will be changed, but the decryption will not change (since
the value of the decryption corresponds exactly to the question of the cypher
being a QR or being QNR).



