\subsection{}
$G'$ is PRG.\\
Proof:\\
Let $G$ be a PRG (with strech $l(n)$).
Denote $S_n=\{1\ldots n\}, R=\{1\ldots l(n)\}$.
Let $\sigma$ be a permutation over $R$.

Assume to contradict that $G:S\longrightarrow R' = <G,\sigma>$ is not PRG.\\
From the definition of PRG, there must be some distinguisher $D'$
with advantage over outputs of $G'$ which are more than $neg(n)$.\\
Namely:
\[
	(*); \exists D: |\pr_{s\leftarrow S_n}[D'(G'(s))=1]
		-\pr_{r\leftarrow R_n}[D'(r)=1]| > neg(n)
\]

We will now use $D'$ to construct a distinguisher $D$:
\[
	(**); D(r)=D'(\sigma(r))
	\Rightarrow D'(r)=D(\sigma^{-1}(r)) 
\]
Note that when we apply a permutation over $R$ to a string of characters,
the meaning is that we produce a new string by reordering the original string
according to the indices generated by the permutation.\\

Given $(*)$ and $(**)$, we can see:
\[
	|\pr_{s\leftarrow S_n}[D'(G'(s))=1]
		-\pr_{r\leftarrow R_n}[D'(r)=1]| > neg(n)\]\[
	\Rightarrow |\pr_{s\leftarrow S_n}[D(\sigma^{-1}(G'(s)))=1]
		-\pr_{r\leftarrow R_n}[D(\sigma(r))=1]| > neg(n)\]\[
	\Rightarrow |\pr_{s\leftarrow S_n}[D(\sigma(\sigma^{-1}(G(s))))=1]
		-\pr_{r\leftarrow R_n}[D(r)=1]| > neg(n)\]\[
	\Rightarrow |\pr_{s\leftarrow S_n}[D(G(s))=1]
		-\pr_{r\leftarrow R_n}[D(r)=1]| > neg(n)	
\]
This is a direct contediction to $G$ being PRG.\\
So there is no distinguisher for $G'$, and the strech condition applies ofcourse
since the permutation does not change the length of output; meaning $G'$ is PRG.

\subsection{}
$G'$ is not PRG.\\
Proof:\\
Take for example the distinguisher $D'$:
$D'(s)=\{s_L=s_R:1, 0\}$, meaning that the distinguisher checks if the left 
half of the input is the same as the right part and if so - returns $1$.\\
Now we can see:
\[
	|\pr_{s\leftarrow S_n}[D'(G'(s))=1]
		-\pr_{r\leftarrow R_n}[D'(r)=1]|\]\[
	= |\pr_{s\leftarrow S_n}[D'(G(s)G(s))=1]
		-\frac{1}{2^{l(n)}}|\]\[
	= |1-\frac{1}{2^{l(n)}}|\approx 1 > neg(n)
\]
Indeed this means $G'$ cannot be PRG.

\subsection{}
$G'$ is PRG.\\
Proof:\\
Assume a distinguisher $D'$ for $G'$.\\
Define $D$:\\
\[
	D(s)=D'(s;r)
\]
where $r$ is sampled from $R$.\\
Since $G$ is PRG, there must be no (distinguishable) statistical 
difference between $r\leftarrow R$ and $G(s):s\leftarrow S$. This means that
for a computationaly limited algorithm such as $D'$, there cannot be a
statistical difference between $D'(G(s);G(s')):s,s'\leftarrow S$ and
$D'(G(s);r):s\leftarrow S, r\leftarrow R$.\\
Hence:
\[
	neg(n)<|\pr_{s\leftarrow S_{2n}}[D'(G'(s))=1]
	-\pr_{r\leftarrow R_{2n}}[D'(r)=1]|\]\[
	=|\pr_{s,s'\leftarrow S_n}[D'(G(s)G(s'))=1]
	-\pr_{r\leftarrow R_n}[D'(r)=1]|\]\[
	=|\pr_{s\leftarrow S_n,r\leftarrow R_n}[D'(G(s);r)=1]
	-\pr_{r\leftarrow R_n}[D'(r)=1]|\]\[
	=|\pr_{s\leftarrow S_n}[D(G(s))=1]
	-\pr_{r\leftarrow R_n}[D(r)=1]|\]\[
\]
But this contredicts $G$ being PGR. So $G'$ must be PRG too (again the strech
condition is trivialy shown).
